trying some NFA inductive characterization

NFA.v
@@ -25,6 +25,59 @@ Definition code : Type := list bytecode.
 Definition get_pc (c:code) (pc:label) : option bytecode :=
   List.nth_error c pc.
 
+Lemma get_prefix:
+  forall c pc prev,
+    get_pc (prev ++ c) (length prev + pc) = get_pc c pc.
+Proof.
+  unfold get_pc. intros.
+  rewrite nth_error_app2; try f_equal; lia.
+Qed.
+
+Corollary get_first:
+  forall c prev,
+    get_pc (prev ++ c) (length prev) = get_pc c 0.
+Proof.
+  intros. replace (length prev) with (length prev + 0) by lia.
+  apply get_prefix.
+Qed.
+
+Corollary get_second:
+  forall c prev,
+    get_pc (prev ++ c) (S (length prev)) = get_pc c 1.
+Proof.
+  intros. replace (S (length prev)) with (length prev + 1) by lia.
+  apply get_prefix.
+Qed.
+
+Corollary get_third:
+  forall c prev,
+    get_pc (prev ++ c) (S (S (length prev))) = get_pc c 2.
+Proof.
+  intros. replace (S (S (length prev))) with (length prev + 2) by lia.
+  apply get_prefix.
+Qed.
+
+Lemma get_suffix:
+  forall c suffix pc i,
+    get_pc c pc = Some i ->
+    get_pc (c++suffix) pc = Some i.
+Proof.
+  unfold get_pc. intros c suffix pc i H.
+  assert (pc < length c).
+  { apply nth_error_Some. rewrite H. unfold not. intros. inversion H0. }
+  rewrite nth_error_app1; auto.
+Qed.
+
+    
+
+
+Definition next_pcs (pc:label) (b:bytecode) : list label :=
+  match b with
+  | Consume _ | SetRegOpen _ | SetRegClose _ | BeginLoop => [S pc]
+  | Accept => []
+  | Jmp l | EndLoop l => [l]
+  | Fork l1 l2 => [l1; l2]
+  end.
 
 (** * NFA Compilation  *)
 
@@ -50,8 +103,61 @@ Fixpoint compile (r:regex) (fresh:label) : code * label :=
       ([SetRegOpen gid] ++ bc1 ++ [SetRegClose gid], S f1)
   end.
 
+(** * Inductive NFA characterization *)
 
+Inductive is_nfa : regex -> code -> label -> label -> Prop :=
+| is_nfa_epsilon:
+  forall c lbl,
+    is_nfa Epsilon c lbl lbl
+| is_nfa_char:
+  forall c cd lbl
+    (CONSUME: get_pc c lbl = Some (Consume cd)),
+    is_nfa (Character cd) c lbl (S lbl)
+| is_nfa_disj:
+  forall c r1 r2 start end1 end2
+    (FORK: get_pc c start = Some (Fork (S start) (S end1)))
+    (NFA1: is_nfa r1 c (S start) end1)
+    (JMP: get_pc c end1 = Some (Jmp end2))
+    (NFA2: is_nfa r2 c (S end1) end2),
+    is_nfa
+      (Disjunction r1 r2) c start end2
+| is_nfa_seq:
+  forall c r1 r2 start end1 end2
+    (NFA1: is_nfa r1 c start end1)
+    (NFA2: is_nfa r2 c end1 end2),
+    is_nfa (Sequence r1 r2) c start end2
+| is_nfa_star:
+  forall c r1 start end1
+    (FORK: get_pc c start = Some (Fork (S start) (S end1)))
+    (BEGIN: get_pc c (S start) = Some (BeginLoop))
+    (NFA1: is_nfa r1 c (S (S start)) end1)
+    (END: get_pc c end1 = Some (EndLoop start)),
+    is_nfa (Star r1) c start (S end1)
+| is_nfa_group:
+  forall c r1 gid start end1
+    (OPEN: get_pc c start = Some (SetRegOpen gid))
+    (NFA1: is_nfa r1 c (S start) end1)
+    (CLOSE: get_pc c end1 = Some (SetRegClose gid)),
+    is_nfa (Group gid r1) c start (S end1).
 
+(** * Compile Characterization  *)
+
+Lemma cons_app:
+  forall A (x:A) l, x::l = [x] ++ l.
+Proof. intros. simpl. auto. Qed.
+
+Lemma is_nfa_extend:
+  forall r c start endl suffix,
+    is_nfa r c start endl ->
+    is_nfa r (c++suffix) start endl.
+Proof.
+  intros r c start endl suffix H. generalize dependent suffix.
+  induction H; intros; econstructor;
+    try (erewrite get_suffix; eauto); try apply IHis_nfa;
+    try apply IHis_nfa1; try apply IHis_nfa2.
+Qed.
+
+(* correctness of the returned fresh label *)
 Lemma fresh_correct:
   forall r fresh l next,
     compile r fresh = (l, next) ->
@@ -76,6 +182,62 @@ Proof.
     destruct (compile r (S fresh)) as [bc1 f1] eqn:COMP1. inversion H0. apply IHr in COMP1.
     subst. simpl. rewrite app_length. simpl. lia.
 Qed.
+
+Theorem compile_is_nfa:
+  forall r c start endl prev,
+    compile r start = (c, endl) ->
+    start = List.length prev ->
+    is_nfa r (prev ++ c) start endl.
+Proof.
+  intros r. induction r; intros.
+  - inversion H. subst. rewrite app_nil_r. constructor.
+  - inversion H. subst. constructor. apply get_first.
+  - inversion H. destruct (compile r1 (S start)) as [bc1 end1] eqn:COMP1. destruct (compile r2 (S end1)) as [bc2 end2] eqn:COMP2.
+    inversion H2. subst. apply is_nfa_disj with (end1:=end1).
+    + rewrite get_first. simpl. auto.
+    + apply IHr1 with (prev:=prev ++ [Fork (S (length prev)) (S end1)]) in COMP1.
+      2: { rewrite app_length. simpl. lia. }
+      replace (prev ++ Fork (S (length prev)) (S end1) :: bc1 ++ Jmp endl :: bc2) with
+        (((prev ++ [Fork (S (length prev)) (S end1)]) ++ bc1) ++ (Jmp endl :: bc2)).
+      2:{ admit. }
+      apply is_nfa_extend. auto.
+    + apply fresh_correct in COMP1. rewrite <- COMP1.
+      replace (S (length prev) + length bc1) with (length prev + (S (length bc1))) by lia.
+      rewrite get_prefix. rewrite cons_app. rewrite app_assoc. apply get_first.
+    + apply IHr2 with (prev:= prev ++ Fork (S (length prev)) (S end1) :: bc1 ++ [Jmp endl]) in COMP2.
+      * replace (prev ++ Fork (S (length prev)) (S end1) :: bc1 ++ Jmp endl :: bc2) with
+          ((prev ++ Fork (S (length prev)) (S end1) :: bc1 ++ [Jmp endl]) ++ bc2).
+        2: { admit. } auto.
+      * apply fresh_correct in COMP1. rewrite <- COMP1. simpl.
+        rewrite app_length. simpl. rewrite app_length. simpl. lia.
+  - (* tedious, but doable *)
+Admitted.
+
+
+
+(* all edges in the code point to valid instructions or the fresh label *)
+Definition code_wf (c:code) (fresh:label) : Prop :=
+  forall pc instr nextpc,
+    get_pc c pc = Some instr ->
+    In nextpc (next_pcs pc instr) ->
+    nextpc = fresh \/ exists instr', get_pc c nextpc = Some instr'.
+
+Lemma empty_wf:
+  forall fresh, code_wf [] fresh.
+Proof.
+  unfold code_wf. intros. unfold get_pc in H. simpl in H. destruct pc; simpl in H; inversion H.
+Qed.
+
+
+Lemma nfa_wf:
+  forall r c start endl,
+    is_nfa r c start endl ->
+    code_wf c endl.
+Proof.
+(* this one isn't true: you could have bogus code before the start.
+ you need a more precise def, to say that code from a certain range is well_formed for a certain range *)
+Admitted.
+          
 
 
 (** * NFA Exponential Semantics  *)
